add bn_mul1

code/bignum/Hacl.Bignum.Base.fst
@@ -62,15 +62,14 @@ let mul_wide_add_t (t:limb_t) =
   Stack (limb t)
   (requires fun h -> live h out)
   (ensures  fun h0 c_out h1 -> modifies (loc out) h0 h1 /\
-    (c_out, LSeq.index (as_seq h1 out) 0) == mul_wide_add a b c_in (LSeq.index (as_seq h0 out) 0))
+    (c_out, LSeq.index (as_seq h1 out) 0) == mul_wide_add a b c_in)
 
 
 val mul_wide_add_u32: mul_wide_add_t U32
 [@CInline]
 let mul_wide_add_u32 a b c_in out =
-  let h0 = ST.get () in
-  lemma_mul_wide_add a b c_in (LSeq.index (as_seq h0 out) 0);
-  let res = to_u64 a *! to_u64 b +! to_u64 c_in +! to_u64 out.(0ul) in
+  lemma_mul_wide_add a b c_in (u32 0);
+  let res = to_u64 a *! to_u64 b +! to_u64 c_in in
   out.(0ul) <- to_u32 res;
   to_u32 (res >>. 32ul)
 
@@ -78,9 +77,8 @@ let mul_wide_add_u32 a b c_in out =
 val mul_wide_add_u64: mul_wide_add_t U64
 [@CInline]
 let mul_wide_add_u64 a b c_in out =
-  let h0 = ST.get () in
-  lemma_mul_wide_add a b c_in (LSeq.index (as_seq h0 out) 0);
-  let res = mul64_wide a b +! to_u128 c_in +! to_u128 out.(0ul) in
+  lemma_mul_wide_add a b c_in (u64 0);
+  let res = mul64_wide a b +! to_u128 c_in in
   out.(0ul) <- to_u64 res;
   to_u64 (res >>. 64ul)
 
@@ -91,3 +89,43 @@ let mul_wide_add_st #t =
   match t with
   | U32 -> mul_wide_add_u32
   | U64 -> mul_wide_add_u64
+
+
+inline_for_extraction noextract
+let mul_wide_add2_t (t:limb_t) =
+    a:limb t
+  -> b:limb t
+  -> c_in:limb t
+  -> out:lbuffer (limb t) 1ul ->
+  Stack (limb t)
+  (requires fun h -> live h out)
+  (ensures  fun h0 c_out h1 -> modifies (loc out) h0 h1 /\
+    (c_out, LSeq.index (as_seq h1 out) 0) == mul_wide_add2 a b c_in (LSeq.index (as_seq h0 out) 0))
+
+
+val mul_wide_add2_u32: mul_wide_add2_t U32
+[@CInline]
+let mul_wide_add2_u32 a b c_in out =
+  let h0 = ST.get () in
+  lemma_mul_wide_add a b c_in (LSeq.index (as_seq h0 out) 0);
+  let res = to_u64 a *! to_u64 b +! to_u64 c_in +! to_u64 out.(0ul) in
+  out.(0ul) <- to_u32 res;
+  to_u32 (res >>. 32ul)
+
+
+val mul_wide_add2_u64: mul_wide_add2_t U64
+[@CInline]
+let mul_wide_add2_u64 a b c_in out =
+  let h0 = ST.get () in
+  lemma_mul_wide_add a b c_in (LSeq.index (as_seq h0 out) 0);
+  let res = mul64_wide a b +! to_u128 c_in +! to_u128 out.(0ul) in
+  out.(0ul) <- to_u64 res;
+  to_u64 (res >>. 64ul)
+
+
+inline_for_extraction noextract
+val mul_wide_add2_st: #t:limb_t -> mul_wide_add2_t t
+let mul_wide_add2_st #t =
+  match t with
+  | U32 -> mul_wide_add2_u32
+  | U64 -> mul_wide_add2_u64
