code/bignum/Hacl.Spec.Bignum.fsti
@@ -123,6 +123,23 @@ val bn_add_mod_n_lemma:
   (ensures  bn_v (bn_add_mod_n n a b) == (bn_v a + bn_v b) % bn_v n)
 
 
+val bn_mul1:
+    #t:limb_t
+  -> #aLen:size_nat
+  -> a:lbignum t aLen
+  -> b1:limb t ->
+  limb t & lbignum t aLen
+
+
+val bn_mul1_lemma:
+    #t:limb_t
+  -> #aLen:size_nat
+  -> a:lbignum t aLen
+  -> b1:limb t ->
+  Lemma (let (c, res) = bn_mul1 a b1 in
+    v c * pow2 (bits t * aLen) + bn_v res == bn_v a * v b1)
+
+
 val bn_mul:
     #t:limb_t
   -> #aLen:size_nat
